Got rid of mutually inductive types

PatternMatchRewrites.v
@@ -14,9 +14,11 @@ Inductive VarName := MkVarName : nat -> VarName.
 
 Inductive CoreType := .
 Scheme Equality for CoreType.
+Hint Resolve CoreType_eq_dec : eqdec.
 
 Inductive Literal := .
 Scheme Equality for Literal.
+Hint Resolve Literal_eq_dec : eqdec.
 
 Inductive Id :=
 | SomeId : VarName -> Id
@@ -42,6 +44,7 @@ Hint Resolve DataCon_dec_eq : eqdec.
 *)
 Inductive DataCon := .
 Scheme Equality for DataCon.
+Hint Resolve DataCon_eq_dec : eqdec.
 
 Inductive AltCon :=
 | DataAlt : DataCon -> AltCon
@@ -54,32 +57,32 @@ Hint Resolve AltCon_dec_eq : eqdec.
 
 Inductive Tickish := .
 Scheme Equality for Tickish.
+Hint Resolve Tickish_eq_dec : eqdec.
 
 Inductive Coercion := .
 Scheme Equality for Coercion.
+Hint Resolve Coercion_eq_dec : eqdec.
 
 Inductive Expr :=
 | Var : Id -> Expr
 | Lit : Literal -> Expr
 | App : Expr -> Expr -> Expr
 | Lam : VarName -> Expr -> Expr
-| Let : Bind -> Expr -> Expr
+(* | Let : ((VarName * Expr) + list (VarName * Expr)) -> Expr -> Expr *)
+| LetNonRec : VarName -> Expr -> Expr -> Expr
+| LetRec : list (VarName * Expr) -> Expr -> Expr
 | Case : Expr -> VarName -> CoreType -> list (AltCon * list VarName * Expr) -> Expr
 | Cast : Expr -> Coercion -> Expr
 | Tick : Tickish -> Expr -> Expr
 | TypeExpr : CoreType -> Expr
-| CoercionExpr : Coercion -> Expr
-
-with Bind :=
-| NonRec : VarName -> Expr -> Bind
-| Rec : list (VarName * Expr) -> Bind.
-
-Scheme Expr_mut := Induction for Expr Sort Prop
-with Bind_mut := Induction for Bind Sort Prop.
-
-Combined Scheme Expr_Bind_mutind from Expr_mut,Bind_mut.
+| CoercionExpr : Coercion -> Expr.
 
 Check fold_right.
+
+Definition Bind := ((VarName * Expr) + list (VarName * Expr)) %type.
+
+Definition NonRec (v : VarName) (e : Expr) : Bind := inl (v, e).
+Definition Rec bs : Bind := inr bs.
 
 Fixpoint Expr_size (e : Expr) : nat :=
   match e with
@@ -87,11 +90,8 @@ Fixpoint Expr_size (e : Expr) : nat :=
   | Lit _ => 1
   | App a b => 1 + Expr_size a + Expr_size b
   | Lam _ x => 1 + Expr_size x
-  | Let bind x =>
-      1 + match bind with
-          | NonRec v b => Expr_size b + Expr_size x
-          | Rec bs => fold_right (fun p q => match p with (_, e) => q + Expr_size e end) 0 bs + Expr_size x
-          end
+  | LetNonRec v b x => 1 + Expr_size b + Expr_size x
+  | LetRec bs x => 1 + fold_right (fun p q => match p with (_, e) => q + Expr_size e end) 0 bs + Expr_size x
 (*
   | Let (NonRec v b) x => 1 + Expr_size b + Expr_size x
   | Let (Rec bs) x => 1 + fold_right (fun p q => match p with (_, e) => q + Expr_size e end) 0 bs + Expr_size x
@@ -104,13 +104,113 @@ Fixpoint Expr_size (e : Expr) : nat :=
   | CoercionExpr _ => 1
   end.
 
+Check list_eq_dec.
 
-Proposition Expr_dec_eq (x y : Expr) : {x=y} + {x<>y}
-with Bind_dec_eq (x y : Bind) : {x=y} + {x<>y}. decide equality; auto with eqdec.
-  repeat decide equality. subst. repeat decide equality. subst. decide equality.
-  repeat (try subst; decide equality). decide equality. decide equality. decide equality.
-  decide equality. decide equality. decide equality. repeat decide equality.
-Defined.
+Program Fixpoint Expr_dec_eq (x y : Expr) : {x=y} + {x<>y} :=
+ltac:(refine
+  match x, y with
+  | Var a, Var b =>
+      match Id_dec_eq a b with
+        | left prf => left (f_equal Var prf)
+        | right prf => right (fun H => _)
+      end
+  | Lit a, Lit b =>
+      match Literal_eq_dec a b with
+        | left prf => left (f_equal Lit prf)
+        | right prf => right (fun H => _)
+      end
+  | App a1 b1, App a2 b2 =>
+      match Expr_dec_eq a1 a2 with
+      | left prf =>
+          match Expr_dec_eq b1 b2 with
+          | left prf2 => left _
+          | right prf2 => right _
+          end
+      | right prf => right _
+      end
+  | Lam v1 e1, Lam v2 e2 =>
+      match VarName_dec_eq v1 v2 with
+      | left prf =>
+          match Expr_dec_eq e1 e2 with
+          | left prf2 => left _
+          | right prf2 => right _
+          end
+      | right prf => right _
+      end
+  | LetNonRec v1 b1 x1, LetNonRec v2 b2 x2 =>
+      match VarName_dec_eq v1 v2 with
+      | left prf =>
+          match Expr_dec_eq b1 b2 with
+          | left prf2 =>
+              match Expr_dec_eq x1 x2 with
+              | left prf3 => left _
+              | right prf3 => right _
+              end
+          | right prf2 => right _
+          end
+      | right prf => right _
+      end
+  | LetRec bs1 x1, LetRec bs2 x2 =>
+      let f := fun p q =>
+          match p, q with
+          | (v1, e1), (v2, e2) =>
+            match VarName_dec_eq v1 v2 with
+            | left prf' =>
+                match Expr_dec_eq e1 e2 with
+                | left prf2' => left _
+                | right prf2' => right _
+                end
+            | right prf' => right _
+            end
+          end
+      in
+      match list_eq_dec f bs1 bs2 with
+      | left prf =>
+          match Expr_dec_eq x1 x2 with
+          | left prf2 => left _
+          | right prf2 => right _
+          end
+      | right prf => right _
+      end
+  | Case s1 wild1 ty1 alts1, Case s2 wild2 ty2 alts2 =>
+      let f := fun p q =>
+          match p, q with
+          | (altCon1, patVars1, e1), (altCon2, patVars2, e2) =>
+            match AltCon_eq_dec altCon1 altCon2 with
+            | left prf' =>
+                match list_eq_dec VarName_dec_eq patVars1 patVars2 with
+                | left prf2' =>
+                    match Expr_dec_eq e1 e2 with
+                    | left prf3' => left _
+                    | right prf3' => right _
+                    end
+                | right prf2' => right _
+                end
+            | right prf' => right _
+            end
+          end
+      in
+      match Expr_dec_eq s1 s2 with
+      | left prf =>
+          match VarName_dec_eq wild1 wild2 with
+          | left prf2 =>
+              match CoreType_eq_dec ty1 ty2 with
+              | left prf3 =>
+                  match list_eq_dec f alts1 alts2 with
+                  | left prf4 => left _
+                  | right prf4 => right _
+                  end
+              | right prf3 => right _
+              end
+          | right prf2 => right _
+          end
+      | right prf => right _
+      end
+  | _, _ => _
+  end).
+Solve All Obligations with try (right; intro; discriminate).
+Solve All Obligations with try (injection H; intro; contradiction).
+Solve All Obligations with try (decide equality; try now decide equality).
 
 Definition Alt : Type := AltCon * list VarName * Expr.
 
@@ -162,7 +262,7 @@ Proof.
   contradiction.
 Defined.
 
-Fixpoint shrinkNotInRecList (v : Id) (x : VarName * Expr) (xs : list (VarName * Expr)) :
+Lemma shrinkNotInRecList (v : Id) (x : VarName * Expr) (xs : list (VarName * Expr)) :
   ~ InRecList v (x :: xs) -> ~ InRecList v xs.
 Proof.
   intros.
@@ -175,6 +275,34 @@ Proof.
   apply InRecList_there. assumption.
   assumption.
 Defined.
+
+Lemma swapNotInRecList (v : Id) (x1 x2 : VarName * Expr) (xs : list (VarName * Expr)) :
+  ~ InRecList v (x1 :: x2 :: xs) -> ~ InRecList v (x2 :: x1 :: xs).
+Proof.
+  intros.
+  intro.
+  case_eq H; intros.
+  destruct x1. destruct x2.
+  destruct (Id_dec_eq v (SomeId v0)); destruct (Id_dec_eq v (SomeId v1)).
+  subst.
+  constructor. reflexivity.
+  assert (A : InRecList v ((v0, e) :: (v1, e0) :: xs)).
+    constructor. assumption.
+  contradiction.
+  assert (A : InRecList v ((v0, e) :: (v1, e0) :: xs)).
+    apply InRecList_there. assumption.
+    constructor. assumption.
+  contradiction.
+  inversion H0. subst.
+  apply InRecList_there. assumption. intuition.
+  subst.
+  inversion H6. subst. intuition.
+  subst.
+  apply InRecList_there. assumption.
+  apply InRecList_there. assumption.
+  assumption.
+Defined.
+
 
 Inductive InVarList : Id -> list VarName -> Prop :=
 | InVarList_cons : forall v v' rest,
@@ -272,7 +400,7 @@ Inductive ReplaceIdWith : Id -> Id -> Expr -> Expr -> Prop :=
        SomeId v = b) /\ 
       rhs' = rhs /\
       body' = body} ->
-    ReplaceIdWith a b (Let (NonRec v rhs) body) (Let (NonRec v rhs') body')
+    ReplaceIdWith a b (LetNonRec v rhs body) (LetNonRec v rhs' body')
 | ReplaceIdWith_Let_Rec : forall a b recList recList' body body',
     {~ InRecList a recList /\
      ~ InRecList b recList /\
@@ -280,7 +408,7 @@ Inductive ReplaceIdWith : Id -> Id -> Expr -> Expr -> Prop :=
      ReplaceIdWith a b body body'}
      +
     {(InRecList a recList \/ InRecList b recList) /\ recList' = recList /\ body' = body} ->
-    ReplaceIdWith a b (Let (Rec recList) body) (Let (Rec recList') body')
+    ReplaceIdWith a b (LetRec recList body) (LetRec recList' body')
 
 | ReplaceIdWith_Case : forall a b s s' wild ty alts alts',
     ReplaceIdWith a b s s' ->
@@ -339,21 +467,21 @@ refine (match e as res return e = res -> _ with
            match ReplaceIdWith_exist a b body _ with
            | existT _ body' prf => existT _ (Lam v body') (ReplaceIdWith_Lam _ _ _ _ _ _)
            end
-  | Let (NonRec v rhs) body => fun Hyp =>
+  | LetNonRec v rhs body => fun Hyp =>
       if Id_dec_eq (SomeId v) a
-      then existT _ (Let (NonRec v rhs) body) (ReplaceIdWith_Let_NonRec _ _ _ _ _ _ _ _)
+      then existT _ (LetNonRec v rhs body) (ReplaceIdWith_Let_NonRec _ _ _ _ _ _ _ _)
       else if Id_dec_eq (SomeId v) b
-           then existT _ (Let (NonRec v rhs) body) (ReplaceIdWith_Let_NonRec _ _ _ _ _ _ _ _)
+           then existT _ (LetNonRec v rhs body) (ReplaceIdWith_Let_NonRec _ _ _ _ _ _ _ _)
            else
              match ReplaceIdWith_exist a b rhs _, ReplaceIdWith_exist a b body _ with
              | existT _ rhs' prf_rhs', existT _ body' prf_body' =>
-                 existT _ (Let (NonRec v rhs') body') (ReplaceIdWith_Let_NonRec _ _ _ _ _ _ _ _)
+                 existT _ (LetNonRec v rhs' body') (ReplaceIdWith_Let_NonRec _ _ _ _ _ _ _ _)
              end
-  | Let (Rec recList) body => fun Hyp =>
+  | LetRec recList body => fun Hyp =>
       if InRecList_dec a recList
-      then existT _ (Let (Rec recList) body) (ReplaceIdWith_Let_Rec _ _ _ _ _ _ _)
+      then existT _ (LetRec recList body) (ReplaceIdWith_Let_Rec _ _ _ _ _ _ _)
       else if InRecList_dec b recList
-           then existT _ (Let (Rec recList) body) (ReplaceIdWith_Let_Rec _ _ _ _ _ _ _)
+           then existT _ (LetRec recList body) (ReplaceIdWith_Let_Rec _ _ _ _ _ _ _)
            else
              let r := ReplaceIdWith_exist a b body _
              in
@@ -365,7 +493,7 @@ refine (match e as res return e = res -> _ with
                  in
                  match m as res3 return m = res3 -> _ with
                  | existT _ recList' prf_recList' => fun Hyp3 =>
-                     existT _ (Let (Rec recList') body') _
+                     existT _ (LetRec recList' body') _
                  end (eq_refl m)
              end (eq_refl r)
   | Case s wild ty alts => fun Hyp =>
@@ -376,7 +504,7 @@ refine (match e as res return e = res -> _ with
             else if Id_dec_eq (SomeId wild) b
                  then existT _ (Case s wild ty alts) (ReplaceIdWith_Case _ _ _ _ _ _ _ _ _ _)
                  else
-                 let prf := _ (* @RelationOnSnd_exists (AltCon * list VarName) _ (ReplaceIdWith a b) (fun e'2 => ReplaceIdWith_exist a b e'2 _) *)
+                 let prf := _ (*@RelationOnSnd_exists (AltCon * list VarName) _ (ReplaceIdWith a b) _ (fun e'2 => ReplaceIdWith_exist a b e'2 _) *)
                  in
                  match MapRelation_exists (RelationOnSnd (ReplaceIdWith a b)) alts prf with
                  | existT _ alts' prf_alts' =>
@@ -423,30 +551,26 @@ Proof.
   exists (TypeExpr c). constructor.
   exists (CoercionExpr c). constructor.
 Unshelve.
-  subst. simpl. intuition.
-  intros.
+  subst. intuition. simpl. intuition.
+  intros.  subst. simpl. intuition.
+  intros.  intuition.
   apply RelationOnSnd_exists.
-  refine (fun a0 e'' prf => ReplaceIdWith_exist a b e'' _).
+  refine (fun a0 e'' prf => ReplaceIdWith_exist a b e'' _). subst.
 
-  rewrite Hyp. rewrite prf in prf0.
-  subst.
   clear Hyp2.
   clear r.
   clear ReplaceIdWith_exist.
   clear n.
   clear n0.
-  induction recList.
-  intuition.
-  pose (P := in_inv prf0).
-  dependent induction P. subst. simpl. intuition.
-
-  subst.
-
-  assert (A : forall z zs, Expr_size (Let (Rec zs) body) < Expr_size (Let (Rec (z :: zs)) body)).
+  induction recList. easy.
+  induction (in_inv prf0). subst.
+  simpl. intuition.
+  pose (IHrecList H).
+  assert (A : forall z zs, Expr_size (LetRec zs body) < Expr_size (LetRec (z :: zs) body)).
     induction zs. simpl.
     intuition.
-    case_eq (Expr_size b1); intros.
-    destruct b1; try ( simpl in H0; discriminate).
+    case_eq (Expr_size b0); intros.
+    destruct b0; try ( simpl in H0; discriminate).
     lia.
 
     simpl.
@@ -455,28 +579,29 @@ Unshelve.
     case_eq (Expr_size e0); intros.
     destruct e0; try (simpl in H0; discriminate).
     lia.
-  pose (IHrecList H).
   subst.
-
-  pose (A' := A a1 recList).
+  pose (A a1 recList).
   lia.
 
   intros.
 
-  apply RelationOnSnd_exists. eapply (fun a0 e'' prf => ReplaceIdWith_exist a b e'' _).
-Unshelve.
-  subst.
-  induction alts. intuition.
-  induction (in_inv prf0). intuition.
+  apply RelationOnSnd_exists.
+  intros.
+  apply ReplaceIdWith_exist. subst.
+  clear n. clear n0.
+  clear prf_s'.
+  clear ReplaceIdWith_exist.
+  clear prf.
+  induction alts. easy.
 
   assert (A : forall z zs, Expr_size (Case s wild ty zs) < Expr_size (Case s wild ty (z :: zs))).
-    induction zs. simpl. intuition.
-    intuition.
+    induction zs. simpl. easy.
+    simpl. easy.
 
-  simpl. intuition.
+  pose (A a0 alts).
+  subst.
+  lia.
 Defined.
-
-Print ReplaceIdWith_exist.
 
 Definition evalReplaceIdWith (a b : Id) (e : Expr) : Expr :=
   match ReplaceIdWith_exist a b e with
@@ -484,6 +609,208 @@ Definition evalReplaceIdWith (a b : Id) (e : Expr) : Expr :=
   end.
 
 Eval cbv in (evalReplaceIdWith RepId UnrepId (App (Var RepId) (Var ConstructId))).
+
+Lemma ReplaceIdWith_det1 : forall a b x x',
+  evalReplaceIdWith a b x = x' ->
+  ReplaceIdWith a b x x'.
+Proof.
+  intros.
+  unfold evalReplaceIdWith in H.
+  destruct (ReplaceIdWith_exist a b x). subst. assumption.
+Defined.
+
+(*
+Lemma evalReplaceIdWith_refl : forall a x,
+  evalReplaceIdWith a a x = x.
+Proof.
+  intros.
+  induction x.
+  - unfold evalReplaceIdWith.
+    induction (ReplaceIdWith_exist a a (Var i)).
+    inversion p. subst. destruct H2. destruct a0. subst. reflexivity.
+    destruct a0. subst. reflexivity.
+
+  - cbv. reflexivity.
+  - unfold evalReplaceIdWith.
+    induction (ReplaceIdWith_exist a a (App x1 x2)).
+    rewrite <- IHx1.
+    rewrite <- IHx2.
+    inversion p. subst.
+(*    unfold evalReplaceIdWith. *)
+    pose (ReplaceIdWith_exist a a x1).
+    inversion s.
+    induction (Expr_dec_eq x x'). subst.
+    rewrite IHx1. rewrite IHx2.
+    induction (Expr_dec_eq f' x1). subst.
+    induction (Expr_dec_eq x' x2). subst.
+    reflexivity.
+    inversion H5; try (subst; (now intuition || (destruct H0; destruct a0; subst; now intuition))).
+    subst. destruct H0. destruct a0. subst. intuition.
+    destruct a0. subst. intuition.
+    subst.
+
+
+
+    fold evalReplaceIdWith.
+    induction (ReplaceIdWith_exist a a x2).
+*)
+
+Program Fixpoint ReplaceIdWith_unchanged (a : Id) (x : Expr) {struct x} :
+  ReplaceIdWith a a x x := _.
+Next Obligation.
+  intros.
+  dependent induction x generalizing x; intros.
+  constructor.
+  destruct (Id_dec_eq i a); now intuition.
+  subst.
+  constructor.
+  subst.
+  constructor; try now assumption.
+  constructor.
+  induction (Id_dec_eq (SomeId v) a); try now intuition.
+
+  case_eq b; intros.
+(*  pose (Let (NonRec v e) x).*)
+  constructor.
+  destruct (Id_dec_eq (SomeId v) a); try now intuition.
+  constructor. constructor. assumption. constructor. assumption.
+  epose (ReplaceIdWith_Let_NonRec a a v e _ x (Let (NonRec v e) x) _).
+  constructor. inversion r. subst. destruct H3.
+  destruct a0. destruct H0. destruct H1. apply H1.
+  destruct a0. intuition.
+  assumption.
+
+  constructor.
+  clear H.
+  induction l.
+  constructor. constructor. intro. inversion H.
+  constructor. intro. inversion H.
+  constructor. constructor. assumption.
+  induction IHl. induction a1. induction H0.
+  induction H1.
+  induction (InRecList_dec a (a0 :: l)).
+  intuition.
+  constructor. constructor. assumption.
+  constructor. assumption.
+  constructor. constructor.
+  destruct a0. constructor.
+  destruct (Id_dec_eq a (SomeId v)).
+  remember b0.
+  induction H1. induction b0.
+  subst.
+  assert (InRecList (SomeId v) ((v, e) :: nil)). constructor. reflexivity.
+  intuition.
+  subst.
+  Check shrinkNotInRecList.
+  Check swapNotInRecList.
+  pose (swapNotInRecList _ _ _ _ b0).
+  pose (shrinkNotInRecList _ _ _ n).
+  pose (shrinkNotInRecList _ _ _ H).
+  pose (IHMapRelation n1 n1 n0 n0 ltac:(reflexivity)).
+  assumption.
+  induction H1.
+
+
+  induction l. induction H1.
+  induction e. intuition.
+  case_eq H1; intros.
+
+  constructor. constructor. intro.
+  destruct a0.
+  induction (Id_dec_eq a (SomeId v)). subst.
+
+
+  destruct (InRecList_dec a (a0 :: l)); try now intuition.
+  constructor. constructor. assumption. constructor. assumption.
+  constructor. subst. clear n.
+  case_eq l; intros. constructor.
+  constructor. destruct p. constructor. subst.
+  
+
+
+  case_eq IHl; intros.
+
+  left. intuition. subst.
+  clear L. clear n.
+  dependent inversion l.
+  constructor.
+  constructor.
+  destruct p.
+  constructor.
+  case_eq IHl; intros.
+
+  destruct IHl. intuition.
+
+Theorem ReplaceIdWith_det : forall a b x x',
+  ReplaceIdWith a b x x' ->
+  evalReplaceIdWith a b x = x'.
+Proof.
+  intros.
+
+  induction H.
+  - destruct H. destruct a0.
+    rewrite H. rewrite H0.
+
+    unfold evalReplaceIdWith.
+    induction (ReplaceIdWith_exist a a' (Var a)).
+    inversion p.
+    destruct H4. destruct a1. subst. intuition. subst. intuition.
+    destruct a0. rewrite H0.
+
+    unfold evalReplaceIdWith.
+    induction (ReplaceIdWith_exist a a' (Var b)).
+    inversion p.
+    destruct H4. destruct a1. subst. intuition. subst.
+    destruct a1. subst. reflexivity.
+
+  - cbv. reflexivity.
+  - destruct H. destruct H. destruct a0.
+    rewrite H. rewrite H1.
+
+    unfold evalReplaceIdWith.
+    induction (ReplaceIdWith_exist a a' (App (Var a) x)).
+    inversion p. subst.
+    inversion H0. destruct H4. destruct a1. subst.
+    inversion H6. destruct H4. destruct a1. subst.
+    inversion H8. destruct H5. destruct a1. subst.
+    reflexivity. intuition. intuition. destruct a1. subst.
+    induction H8. destruct H1. destruct a0. subst.
+    
+    rewrite IHReplaceIdWith1.
+(*    pose (Q := ReplaceIdWith_det1 a a' x (evalReplaceIdWith a a' x) ltac:(reflexivity)). *)
+    inversion H0. subst. destruct H. destruct a0.
+
+
+
+
+
+  induction x; inversion H; subst.
+  destruct H3. destruct a0. subst.
+  unfold evalReplaceIdWith.
+  induction (ReplaceIdWith_exist a b (Var a)).
+  induction p. destruct H0. destruct a0. subst.
+  reflexivity. destruct a0. subst.
+
+Theorem ReplaceIdWith_confluent : forall a b x x1' x2',
+  ReplaceIdWith a b x x1' ->
+  ReplaceIdWith a b x x2' ->
+  x1' = x2'.
+Proof.
+  intros.
+
+  induction H; inversion H0; try (subst; intuition; subst; now intuition).
+  subst.
+
+  
+
+  case_eq H0; intros.
+  destruct s. destruct a1. subst.
+
+  induction H; try (epose (IHReplaceIdWith1 _); discriminate).
+
+
+  induction H6. intuition. subst.
+  inversion H6. subst. intuition. subst.
 
 
 Inductive HasExternalize : Expr -> Prop :=
@@ -499,7 +826,7 @@ Inductive HasExternalize : Expr -> Prop :=
     HasExternalize (Case s wild ty (cons (altcon, patVars, rhs) restAlts))
 | HasExternalize_Cast : forall e co,
     HasExternalize e -> HasExternalize (Cast e co)
-| HasExternalizee_Tick : forall t e,
+| HasExternalize_Tick : forall t e,
     HasExternalize e -> HasExternalize (Tick t e)
 
 with HasExternalizeBind : Bind -> Prop :=
